Add simpler version of verification helpers
Assumes that assumptions on traces that we want to consider are given as
predicates on individual events that must hold for all events in the
trace, rather than as predicates on full traces.  This should still
allow us to capture many of the assumptions we need (e.g. that the
capability in all register read events from PCC in instruction traces is
unsealed) while disentangling the proof of the T-CHERI properties and
the proof of ISA invariants, potentially simplifying both parts of the
proof.

model/Recognising_Automata.thy
@@ -892,6 +892,449 @@ qed
 
 end
 
+locale Cap_Axiom_Assm_Automaton = Cap_Axiom_Automaton CC ISA enabled
+  for CC :: "'cap Capability_class" and ISA :: "('cap, 'regval, 'instr, 'e) isa"
+    and enabled :: "('cap, 'regval) axiom_state \<Rightarrow> 'regval event \<Rightarrow> bool" +
+  fixes ex_traces :: bool
+    and ev_assms :: "'regval event \<Rightarrow> bool"
+  assumes non_cap_event_enabled: "\<And>e. non_cap_event e \<Longrightarrow> enabled s e"
+    and read_non_special_regs_enabled: "\<And>r v. r \<notin> PCC ISA \<union> IDC ISA \<union> KCC ISA \<union> privileged_regs ISA \<Longrightarrow> enabled s (E_read_reg r v)"
+begin
+
+definition "trace_assms t \<equiv> \<forall>e \<in> set t. ev_assms e"
+
+lemma trace_assms_append[iff]: "trace_assms (t1 @ t2) \<longleftrightarrow> trace_assms t1 \<and> trace_assms t2"
+  by (auto simp: trace_assms_def)
+
+definition "isException m \<equiv> ((\<exists>e. m = Exception e) \<or> (\<exists>msg. m = Fail msg)) \<and> ex_traces"
+
+definition finished :: "('regval,'a,'ex) monad \<Rightarrow> bool" where
+  "finished m = ((\<exists>a. m = Done a) \<or> isException m)"
+
+lemma finishedE:
+  assumes "finished m"
+  obtains (Done) a where "m = Done a"
+  | (Ex) "isException m"
+  using assms
+  by (auto simp: finished_def)
+
+lemma finished_cases:
+  assumes "finished m"
+  obtains (Done) a where "m = Done a" | (Fail) msg where "m = Fail msg" | (Ex) e where "m = Exception e"
+  using assms
+  by (auto simp: finished_def isException_def)
+
+lemma finished_Done[intro, simp]:
+  "finished (Done a)"
+  by (auto simp: finished_def)
+
+lemma finished_Fail[intro, simp]:
+  "finished (Fail msg) \<Longrightarrow> finished (Fail msg')"
+  unfolding finished_def isException_def
+  by auto
+
+lemma finished_Exception[intro, simp]:
+  "finished (Exception e) \<Longrightarrow> finished (Exception e')"
+  unfolding finished_def isException_def
+  by auto
+
+lemma finished_isException[intro, simp]:
+  "isException m \<Longrightarrow> finished m"
+  by (auto simp: finished_def)
+
+lemma finished_bind_left:
+  assumes "finished (m \<bind> f)"
+  shows "finished m"
+  using assms
+  unfolding finished_def isException_def
+  by (cases m) auto
+
+definition
+  "traces_enabled m s \<equiv>
+     \<forall>t m'. (m, t, m') \<in> Traces \<and> finished m' \<and> trace_assms t \<longrightarrow> trace_enabled s t"
+
+lemma traces_enabled_accepts_fromI:
+  assumes "hasTrace t m" and "traces_enabled m s" and "hasException t m \<or> hasFailure t m \<longrightarrow> ex_traces"
+    and "trace_assms t"
+  shows "accepts_from s t"
+  using assms
+  unfolding traces_enabled_def finished_def isException_def
+  unfolding hasTrace_iff_Traces_final hasException_iff_Traces_Exception hasFailure_iff_Traces_Fail
+  unfolding runTrace_iff_Traces[symmetric]
+  by (intro trace_enabled_acceptI) (auto elim!: final_cases)
+
+named_theorems traces_enabledI
+
+lemma traces_enabled_bind[traces_enabledI]:
+  assumes "traces_enabled m s"
+    and "\<And>t a. Run m t a \<Longrightarrow> trace_assms t \<Longrightarrow> traces_enabled (f a) (run s t)"
+  shows "traces_enabled (m \<bind> f) s"
+  using assms
+  by (auto simp: traces_enabled_def trace_enabled_append_iff
+      elim!: bind_Traces_cases dest!: finished_bind_left;
+      fastforce)
+
+lemma non_cap_trace_enabledI:
+  assumes "non_cap_trace t"
+  shows "trace_enabled s t"
+  using assms
+  by (induction t) (auto simp: non_cap_event_enabled non_cap_event_axiom_step_inv)
+
+lemma non_cap_exp_trace_enabledI:
+  assumes m: "non_cap_exp m"
+    and t: "(m, t, m') \<in> Traces"
+  shows "trace_enabled s t"
+  by (cases rule: non_cap_exp_Traces_cases[OF m t])
+     (auto intro: non_cap_trace_enabledI read_non_special_regs_enabled simp: trace_enabled_append_iff)
+
+lemma non_cap_exp_traces_enabledI:
+  assumes "non_cap_exp m"
+  shows "traces_enabled m s"
+  using assms
+  by (auto simp: traces_enabled_def intro: non_cap_exp_trace_enabledI)
+
+lemma traces_enabled_let[traces_enabledI]:
+  assumes "traces_enabled (f y) s"
+  shows "traces_enabled (let x = y in f x) s"
+  using assms
+  by auto
+
+lemma traces_enabled_case_prod[traces_enabledI]:
+  assumes "\<And>x y. z = (x, y) \<Longrightarrow> traces_enabled (f x y) s"
+  shows "traces_enabled (case z of (x, y) \<Rightarrow> f x y) s"
+  using assms
+  by auto
+
+lemma traces_enabled_if[traces_enabledI]:
+  assumes "c \<Longrightarrow> traces_enabled m1 s" and "\<not>c \<Longrightarrow> traces_enabled m2 s"
+  shows "traces_enabled (if c then m1 else m2) s"
+  using assms
+  by auto
+
+lemma traces_enabled_if_ignore_cond:
+  assumes "traces_enabled m1 s" and "traces_enabled m2 s"
+  shows "traces_enabled (if c then m1 else m2) s"
+  using assms
+  by auto
+
+lemma traces_enabled_and_boolM[traces_enabledI]:
+  assumes "traces_enabled m1 s"
+    and "\<And>t. Run m1 t True \<Longrightarrow> traces_enabled m2 (run s t)"
+  shows "traces_enabled (and_boolM m1 m2) s"
+  using assms
+  by (auto simp: and_boolM_def intro!: traces_enabledI intro: non_cap_exp_traces_enabledI non_cap_expI)
+
+lemma traces_enabled_or_boolM[traces_enabledI]:
+  assumes "traces_enabled m1 s"
+    and "\<And>t. Run m1 t False \<Longrightarrow> traces_enabled m2 (run s t)"
+  shows "traces_enabled (or_boolM m1 m2) s"
+  using assms
+  by (auto simp: or_boolM_def intro!: traces_enabledI intro: non_cap_exp_traces_enabledI non_cap_expI)
+
+lemma traces_enabled_foreachM_inv:
+  assumes "\<And>x vars s. P vars s \<Longrightarrow> x \<in> set xs \<Longrightarrow> traces_enabled (body x vars) s"
+    and "\<And>x vars s t vars'. P vars s \<Longrightarrow> x \<in> set xs \<Longrightarrow> Run (body x vars) t vars' \<Longrightarrow> P vars' (run s t)"
+    and "P vars s"
+  shows "traces_enabled (foreachM xs vars body) s"
+  by (use assms in \<open>induction xs arbitrary: vars s\<close>;
+      fastforce intro!: traces_enabledI intro: non_cap_exp_traces_enabledI non_cap_expI)
+
+lemma traces_enabled_try_catch:
+  assumes "traces_enabled m s"
+    and "\<And>tm e th m'.
+           \<lbrakk>(m, tm, Exception e) \<in> Traces; (h e, th, m') \<in> Traces; finished m'; trace_assms tm\<rbrakk> \<Longrightarrow>
+           trace_enabled s (tm @ th)"
+  shows "traces_enabled (try_catch m h) s"
+proof -
+  have *: "finished (try_catch m h) \<longleftrightarrow> (\<exists>a. m = Done a) \<or> (\<exists>msg. m = Fail msg \<and> finished m) \<or> (\<exists>e. m = Exception e \<and> (h e, [], h e) \<in> Traces \<and> finished (h e))" for m
+    by (cases m) (auto simp: finished_def isException_def)
+  show ?thesis
+    using assms
+    by (fastforce simp: traces_enabled_def trace_enabled_append_iff * elim!: try_catch_Traces_cases)
+qed
+
+lemma traces_enabled_liftR[traces_enabledI]:
+  assumes "traces_enabled m s"
+  shows "traces_enabled (liftR m) s"
+  using assms
+  unfolding liftR_def
+  by (intro traces_enabled_try_catch) (auto simp: traces_enabled_def)
+
+definition
+  "early_returns_enabled m s \<equiv>
+     traces_enabled m s \<and>
+     (\<forall>t a. (m, t, Exception (Inl a)) \<in> Traces \<and> trace_assms t \<longrightarrow> trace_enabled s t)"
+
+lemma traces_enabled_catch_early_return[traces_enabledI]:
+  assumes "early_returns_enabled m s"
+  shows "traces_enabled (catch_early_return m) s"
+  using assms
+  unfolding catch_early_return_def
+  by (intro traces_enabled_try_catch)
+     (auto simp: traces_enabled_def early_returns_enabled_def split: sum.splits)
+
+lemma liftR_no_early_return[simp]:
+  shows "(liftR m, t, Exception (Inl e)) \<in> Traces \<longleftrightarrow> False"
+  by (induction m arbitrary: t) (auto simp: liftR_def elim: Traces_cases)
+
+lemma early_returns_enabled_liftR[traces_enabledI]:
+  assumes "traces_enabled m s"
+  shows "early_returns_enabled (liftR m) s"
+  using assms
+  by (auto simp: early_returns_enabled_def intro: traces_enabled_liftR)
+
+lemma early_returns_enabled_return[traces_enabledI]:
+  "early_returns_enabled (return a) s"
+  by (auto simp: early_returns_enabled_def traces_enabled_def)
+
+lemma early_returns_enabled_bind[traces_enabledI]:
+  assumes m: "early_returns_enabled m s"
+    and f: "\<And>t a. Run m t a \<Longrightarrow> trace_assms t \<Longrightarrow> early_returns_enabled (f a) (run s t)"
+  shows "early_returns_enabled (m \<bind> f) s"
+proof -
+  { fix t a
+    assume "(m \<bind> f, t, Exception (Inl a)) \<in> Traces" and t: "trace_assms t"
+    then have "trace_enabled s t"
+    proof (cases rule: bind_Traces_cases)
+      case (Left m'')
+      then consider "m'' = Exception (Inl a)" | a' where "m'' = Done a'" and "f a' = Exception (Inl a)"
+        by (cases m'') auto
+      then show ?thesis
+        using Left m t
+        by cases (auto simp: early_returns_enabled_def traces_enabled_def)
+    next
+      case (Bind tm am tf)
+      then show ?thesis
+        using Bind m f[of tm am] t
+        by (auto simp: trace_enabled_append_iff early_returns_enabled_def traces_enabled_def)
+    qed
+  }
+  then show ?thesis
+    using assms
+    by (auto intro: traces_enabled_bind simp: early_returns_enabled_def)
+qed
+
+lemma early_returns_enabled_early_return[traces_enabledI]:
+  "early_returns_enabled (early_return a) s"
+  by (auto simp: early_returns_enabled_def early_return_def throw_def traces_enabled_def)
+
+lemma early_returns_enabled_let[traces_enabledI]:
+  assumes "early_returns_enabled (f y) s"
+  shows "early_returns_enabled (let x = y in f x) s"
+  using assms
+  by auto
+
+lemma early_returns_enabled_case_prod[traces_enabledI]:
+  assumes "\<And>x y. z = (x, y) \<Longrightarrow> early_returns_enabled (f x y) s"
+  shows "early_returns_enabled (case z of (x, y) \<Rightarrow> f x y) s"
+  using assms
+  by auto
+
+lemma early_returns_enabled_if[traces_enabledI]:
+  assumes "c \<Longrightarrow> early_returns_enabled m1 s" and "\<not>c \<Longrightarrow> early_returns_enabled m2 s"
+  shows "early_returns_enabled (if c then m1 else m2) s"
+  using assms
+  by auto
+
+lemma early_returns_enabled_if_ignore_cond:
+  assumes "early_returns_enabled m1 s" and "early_returns_enabled m2 s"
+  shows "early_returns_enabled (if c then m1 else m2) s"
+  using assms
+  by auto
+
+lemma early_returns_enabled_and_boolM[traces_enabledI]:
+  assumes "early_returns_enabled m1 s"
+    and "\<And>t. Run m1 t True \<Longrightarrow> early_returns_enabled m2 (run s t)"
+  shows "early_returns_enabled (and_boolM m1 m2) s"
+  using assms
+  by (auto simp: and_boolM_def intro!: traces_enabledI intro: non_cap_exp_traces_enabledI non_cap_expI)
+
+lemma early_returns_enabled_or_boolM[traces_enabledI]:
+  assumes "early_returns_enabled m1 s"
+    and "\<And>t. Run m1 t False \<Longrightarrow> early_returns_enabled m2 (run s t)"
+  shows "early_returns_enabled (or_boolM m1 m2) s"
+  using assms
+  by (auto simp: or_boolM_def intro!: traces_enabledI intro: non_cap_exp_traces_enabledI non_cap_expI)
+
+lemma early_returns_enabled_foreachM_inv:
+  assumes "\<And>x vars s. P vars s \<Longrightarrow> x \<in> set xs \<Longrightarrow> early_returns_enabled (body x vars) s"
+    and "\<And>x vars s t vars'. P vars s \<Longrightarrow> x \<in> set xs \<Longrightarrow> Run (body x vars) t vars' \<Longrightarrow> P vars' (run s t)"
+    and "P vars s"
+  shows "early_returns_enabled (foreachM xs vars body) s"
+  by (use assms in \<open>induction xs arbitrary: vars s\<close>;
+      fastforce intro!: traces_enabledI intro: non_cap_exp_traces_enabledI non_cap_expI)
+
+lemma non_cap_exp_Run_inv_traces_enabled_runE:
+  assumes "Run m1 t a" and "non_cap_exp m1" and "traces_enabled m2 s"
+  shows "traces_enabled m2 (run s t)"
+  using assms
+  by (auto simp: non_cap_exp_Run_run_invI)
+
+lemma non_cap_exp_Run_inv_early_returns_enabled_runE:
+  assumes "Run m1 t a" and "non_cap_exp m1" and "early_returns_enabled m2 s"
+  shows "early_returns_enabled m2 (run s t)"
+  using assms
+  by (auto simp: non_cap_exp_Run_run_invI)
+
+lemma accessible_regs_no_writes_run:
+  assumes t: "Run m t a"
+    and m: "runs_no_reg_writes_to {r} m"
+    and s: "r \<in> accessible_regs s"
+  shows "r \<in> accessible_regs (run s t)"
+proof -
+  have no_write: "\<forall>v. E_write_reg r v \<notin> set t"
+    using m t
+    by (auto simp: runs_no_reg_writes_to_def)
+  show ?thesis
+  proof (use s no_write in \<open>induction t arbitrary: s\<close>)
+    case (Cons e t)
+    then have "r \<in> accessible_regs (axiom_step s e)" and "\<forall>v. E_write_reg r v \<notin> set t"
+      by (auto simp: accessible_regs_def)
+    from Cons.IH[OF this] show ?case by auto
+  qed auto
+qed
+
+lemma no_reg_writes_to_mono:
+  assumes "runs_no_reg_writes_to Rs m"
+    and "Rs' \<subseteq> Rs"
+  shows "runs_no_reg_writes_to Rs' m"
+  using assms
+  by (auto simp: runs_no_reg_writes_to_def)
+
+lemma accessible_regs_no_writes_run_subset:
+  assumes t: "Run m t a" and m: "runs_no_reg_writes_to Rs m"
+    and Rs: "Rs \<subseteq> accessible_regs s"
+  shows "Rs \<subseteq> accessible_regs (run s t)"
+  using t Rs no_reg_writes_to_mono[OF m]
+  by (auto intro: accessible_regs_no_writes_run)
+
+(*method accessible_regsI uses simp assms =
+  (match conclusion in \<open>Rs \<subseteq> accessible_regs (run s t)\<close> for Rs s t \<Rightarrow>
+     \<open>match premises in t: \<open>Run_inv m t a regs\<close> for m a regs \<Rightarrow>
+        \<open>rule accessible_regs_no_writes_run_subset[OF t],
+         solves \<open>use assms in \<open>no_reg_writes_toI simp: simp\<close>,
+         accessible_regsI simp: simp assms: assms\<close>\<close>\<close>
+   \<bar> \<open>Rs \<subseteq> accessible_regs s\<close> for Rs s \<Rightarrow> \<open>use assms in \<open>auto simp: simp\<close>\<close>)*)
+
+named_theorems accessible_regsE
+named_theorems accessible_regsI
+
+method accessible_regs_step uses simp assms =
+  ((erule accessible_regsE eqTrueE)
+    | (rule accessible_regsI TrueI)
+    | (erule accessible_regs_no_writes_run_subset,
+       solves \<open>use assms in \<open>no_reg_writes_toI simp: simp\<close>\<close>))
+
+method accessible_regsI_with methods solve uses simp assms =
+  ((erule accessible_regsE eqTrueE; accessible_regsI_with solve simp: simp assms: assms)
+    | (rule accessible_regsI TrueI; accessible_regsI_with solve simp: simp assms: assms)
+    | (erule accessible_regs_no_writes_run_subset,
+       solves \<open>use assms in \<open>no_reg_writes_toI simp: simp\<close>\<close>,
+       accessible_regsI_with solve simp: simp assms: assms)
+    | solve)
+
+method accessible_regsI uses simp assms =
+  (accessible_regsI_with
+     \<open>(use assms in \<open>no_reg_writes_toI simp: simp\<close>)
+       | (use assms in \<open>auto simp: simp\<close>)\<close>
+     simp: simp assms: assms)
+
+definition "derivable_caps s \<equiv> {c. is_tagged_method CC c \<longrightarrow> c \<in> derivable (accessed_caps s)}"
+
+named_theorems derivable_capsI
+named_theorems derivable_capsE
+
+lemma accessed_caps_run_mono:
+  "accessed_caps s \<subseteq> accessed_caps (run s t)"
+  by (rule subsetI) (induction t arbitrary: s; auto)
+
+lemma derivable_caps_run_mono:
+  "derivable_caps s \<subseteq> derivable_caps (run s t)"
+  using derivable_mono[OF accessed_caps_run_mono]
+  by (auto simp: derivable_caps_def)
+
+lemma derivable_caps_run_imp:
+  "c \<in> derivable_caps s \<Longrightarrow> c \<in> derivable_caps (run s t)"
+  using derivable_caps_run_mono
+  by auto
+
+method derivable_caps_step =
+  (rule derivable_capsI TrueI
+      | erule derivable_capsE eqTrueE
+      | rule derivable_caps_run_imp)
+
+method derivable_capsI_with methods solve uses intro elim simp assms =
+  ((rule intro derivable_capsI TrueI
+      | erule elim derivable_capsE eqTrueE
+      | rule derivable_caps_run_imp
+      | solve (*
+      | solves \<open>use assms in \<open>auto simp: simp\<close>\<close>*));
+   derivable_capsI_with solve intro: intro elim: elim simp: simp assms: assms)
+
+method derivable_capsI uses intro elim simp assms =
+  (derivable_capsI_with
+     \<open>(solves \<open>accessible_regsI simp: simp assms: assms\<close>)\<close>
+     intro: intro elim: elim simp: simp assms: assms)
+
+method try_simp_traces_enabled =
+  ((match conclusion in \<open>traces_enabled m2 (run s t)\<close> for m2 s t \<Rightarrow>
+     \<open>match premises in m1: \<open>Run m1 t a\<close> for m1 a \<Rightarrow>
+        \<open>(rule non_cap_exp_Run_inv_traces_enabled_runE[OF m1], solves \<open>non_cap_expI\<close>)?\<close>\<close>
+   \<bar> \<open>early_returns_enabled m2 (run s t)\<close> for m2 s t \<Rightarrow>
+     \<open>match premises in m1: \<open>Run m1 t a\<close> for m1 a \<Rightarrow>
+        \<open>(rule non_cap_exp_Run_inv_early_returns_enabled_runE[OF m1], solves \<open>non_cap_expI\<close>)?\<close>\<close>)?)
+
+named_theorems traces_enabled_combinatorI
+
+lemmas traces_enabled_builtin_combinatorsI =
+  traces_enabled_bind traces_enabled_and_boolM traces_enabled_or_boolM
+  early_returns_enabled_bind early_returns_enabled_and_boolM early_returns_enabled_or_boolM
+
+named_theorems traces_enabled_split
+declare option.split[where P = "\<lambda>m. traces_enabled m s" for s, traces_enabled_split]
+declare prod.split[where P = "\<lambda>m. traces_enabled m s" for s, traces_enabled_split]
+declare sum.split[where P = "\<lambda>m. traces_enabled m s" for s, traces_enabled_split]
+declare bool.split[where P = "\<lambda>m. traces_enabled m s" for s, traces_enabled_split]
+
+method traces_enabled_step uses intro elim =
+  ((rule intro TrueI)
+    | (erule elim eqTrueE)
+    | ((rule traces_enabled_combinatorI traces_enabled_builtin_combinatorsI[rotated], try_simp_traces_enabled))
+    | (rule traces_enabled_split[THEN iffD2]; intro allI conjI impI))
+
+method traces_enabledI_with methods solve uses intro elim =
+  ((rule intro TrueI; traces_enabledI_with solve intro: intro elim: elim)
+    | (erule elim eqTrueE; traces_enabledI_with solve intro: intro elim: elim)
+    | ((rule traces_enabled_combinatorI traces_enabled_builtin_combinatorsI[rotated], try_simp_traces_enabled); traces_enabledI_with solve intro: intro elim: elim)
+    | (rule traces_enabledI; traces_enabledI_with solve intro: intro elim: elim)
+    | (rule traces_enabled_split[THEN iffD2]; intro conjI impI; traces_enabledI_with solve intro: intro elim: elim)
+    | solve)
+
+(*method traces_enabledI uses simp intro elim assms =
+  (traces_enabledI_with
+     \<open>(solves \<open>accessible_regsI simp: simp assms: assms\<close>)
+      | (solves \<open>derivable_capsI simp: simp assms: assms\<close>)
+      | (use assms in \<open>auto intro!: intro elim!: elim simp: simp\<close>)?\<close>
+     intro: intro)*)
+
+method traces_enabledI uses simp intro elim assms =
+  ((traces_enabled_step intro: intro elim: elim; traces_enabledI simp: simp intro: intro elim: elim assms: assms)
+    | (accessible_regs_step simp: simp assms: assms; solves \<open>traces_enabledI simp: simp intro: intro elim: elim assms: assms\<close>)
+    | (derivable_caps_step; solves \<open>traces_enabledI simp: simp intro: intro elim: elim assms: assms\<close>)
+    | (solves \<open>no_reg_writes_toI simp: simp\<close>)
+    | (use assms in \<open>auto intro!: intro elim!: elim simp: simp\<close>)?)
+
+(* method traces_enabledI = (intro traces_enabledI preserves_invariantI) *)
+
+lemma if_derivable_capsI[derivable_capsI]:
+  assumes "cond \<Longrightarrow> c1 \<in> derivable_caps s" and "\<not>cond \<Longrightarrow> c2 \<in> derivable_caps s"
+  shows "(if cond then c1 else c2) \<in> derivable_caps s"
+  using assms
+  by auto
+
+
+end
+
 locale Cap_Axiom_Inv_Automaton = Cap_Axiom_Automaton CC ISA enabled +
   State_Invariant get_regval set_regval invariant inv_regs
   for CC :: "'cap Capability_class" and ISA :: "('cap, 'regval, 'instr, 'e) isa"
@@ -1378,6 +1821,68 @@ lemma if_derivable_capsI[derivable_capsI]:
 
 end
 
+locale Write_Cap_Assm_Automaton =
+  Write_Cap_Automaton CC ISA ex_traces invoked_caps
+  for CC :: "'cap Capability_class" and ISA :: "('cap, 'regval, 'instr, 'e) isa"
+  and ex_traces :: bool and invoked_caps :: "'cap set" +
+  fixes ev_assms :: "'regval event \<Rightarrow> bool"
+begin
+
+sublocale Cap_Axiom_Assm_Automaton where enabled = enabled
+proof
+  fix s e
+  assume "non_cap_event e"
+  then show "enabled s e"
+    by (cases e) auto
+next
+  fix s r v
+  assume "r \<notin> special_reg_names"
+  then show "enabled s (E_read_reg r v)"
+    by auto
+qed
+
+lemma read_reg_trace_enabled:
+  assumes t: "(read_reg r, t, m') \<in> Traces"
+    and r: "name r \<in> privileged_regs ISA \<longrightarrow> system_reg_access s \<or> ex_traces"
+  shows "trace_enabled s t"
+  by (use t in \<open>auto simp: read_reg_def elim!: Read_reg_TracesE split: option.splits\<close>)
+     (use r in \<open>auto\<close>)
+
+lemma traces_enabled_read_reg:
+  assumes "name r \<in> privileged_regs ISA \<longrightarrow> (system_reg_access s \<or> ex_traces)"
+  shows "traces_enabled (read_reg r) s"
+  using assms
+  unfolding traces_enabled_def
+  by (blast intro: read_reg_trace_enabled)
+
+lemma write_reg_trace_enabled:
+  assumes "(write_reg r v, t, m') \<in> Traces"
+    and "enabled s (E_write_reg (name r) (regval_of r v))"
+  shows "trace_enabled s t"
+  using assms
+  by (auto simp add: write_reg_def simp del: enabled.simps elim!: Write_reg_TracesE)
+
+lemma traces_enabled_write_reg:
+  assumes "enabled s (E_write_reg (name r) (regval_of r v))"
+  shows "traces_enabled (write_reg r v) s"
+  using assms
+  unfolding traces_enabled_def
+  by (blast intro: write_reg_trace_enabled)
+
+lemma traces_enabled_reg_axioms:
+  assumes "traces_enabled m initial" and "hasTrace t m"
+    and "trace_assms t"
+    and "hasException t m \<or> hasFailure t m \<longrightarrow> ex_traces"
+  shows "store_cap_reg_axiom CC ISA ex_traces invoked_caps t"
+    and "store_cap_mem_axiom CC ISA t"
+    and "read_reg_axiom CC ISA ex_traces t"
+  using assms
+  by (intro recognises_store_cap_reg_read_reg_axioms;
+      elim traces_enabled_accepts_fromI;
+      auto)+
+
+end
+
 locale Write_Cap_Inv_Automaton =
   Write_Cap_Automaton CC ISA ex_traces invoked_caps +
   State_Invariant get_regval set_regval invariant inv_regs
@@ -1445,8 +1950,8 @@ end
 
 locale Capability_ISA_Fixed_Translation = Capability_ISA CC ISA
   for CC :: "'cap Capability_class" and ISA :: "('cap, 'regval, 'instr, 'e) isa" +
-  fixes translation_assm :: "'regval trace \<Rightarrow> bool"
-  assumes fixed_translation: "\<And>i t addr load. translation_assm t \<Longrightarrow> translate_address ISA addr load (take i t) = translate_address ISA addr load []"
+  fixes translation_assms :: "'regval trace \<Rightarrow> bool"
+  assumes fixed_translation: "\<And>i t addr load. translation_assms t \<Longrightarrow> translate_address ISA addr load (take i t) = translate_address ISA addr load []"
 
 fun non_store_event :: "'regval event \<Rightarrow> bool" where
   "non_store_event (E_write_mem _ paddr sz v _) = False"
@@ -1539,7 +2044,7 @@ fun enabled :: "('cap, 'regval) axiom_state \<Rightarrow> 'regval event \<Righta
 sublocale Cap_Axiom_Automaton where enabled = enabled ..
 
 lemma accepts_store_mem_axiom:
-  assumes *: "translation_assm t" and  **: "accepts t"
+  assumes *: "translation_assms t" and  **: "accepts t"
   shows "store_mem_axiom CC ISA t"
   using accepts_from_nth_enabledI[OF **]
   unfolding store_mem_axiom_def
@@ -1556,7 +2061,7 @@ lemma accepts_store_tag_axiom:
   by (fastforce simp: access_enabled_defs bind_eq_Some_conv Let_def elim!: writes_mem_val.elims)
 
 lemma accepts_load_mem_axiom:
-  assumes *: "translation_assm t" and  **: "accepts t"
+  assumes *: "translation_assms t" and  **: "accepts t"
   shows "load_mem_axiom CC ISA is_fetch t"
   unfolding load_mem_axiom_def
   unfolding reads_mem_val_at_idx_def cap_derivable_iff_derivable
@@ -1577,11 +2082,57 @@ lemma non_mem_trace_enabledI:
 
 end
 
+locale Mem_Assm_Automaton =
+  Mem_Automaton translation_assms CC ISA is_fetch
+  for CC :: "'cap Capability_class" and ISA :: "('cap, 'regval, 'instr, 'e) isa"
+    and translation_assms :: "'regval event list \<Rightarrow> bool"
+    and is_fetch :: bool and ex_traces :: bool +
+  fixes ev_assms :: "'regval event \<Rightarrow> bool"
+begin
+
+sublocale Cap_Axiom_Assm_Automaton where enabled = enabled and ex_traces = ex_traces
+proof
+  fix s e
+  assume "non_cap_event e"
+  then show "enabled s e"
+    by (cases e) auto
+next
+  fix s r v
+  assume "r \<notin> special_reg_names"
+  then show "enabled s (E_read_reg r v)"
+    by auto
+qed
+
+lemma non_mem_exp_trace_enabledI:
+  "trace_enabled s t" if "non_mem_exp m" and "(m, t, m') \<in> Traces"
+  using that
+  by (auto simp: non_mem_exp_def intro: non_mem_trace_enabledI)
+
+lemma non_mem_exp_traces_enabledI:
+  "traces_enabled m s" if "non_mem_exp m"
+  using that
+  by (auto simp: traces_enabled_def intro: non_mem_exp_trace_enabledI)
+
+lemma traces_enabled_mem_axioms:
+  assumes "traces_enabled m initial" and "hasTrace t m"
+    and "trace_assms t"
+    and "hasException t m \<or> hasFailure t m \<longrightarrow> ex_traces"
+    and "translation_assms t"
+  shows "store_mem_axiom CC ISA t"
+    and "store_tag_axiom CC ISA t"
+    and "load_mem_axiom CC ISA is_fetch t"
+  using assms
+  by (intro accepts_store_mem_axiom accepts_store_tag_axiom accepts_load_mem_axiom
+            traces_enabled_accepts_fromI;
+      auto)+
+
+end
+
 locale Mem_Inv_Automaton =
-  Mem_Automaton translation_assm CC ISA is_fetch +
+  Mem_Automaton translation_assms CC ISA is_fetch +
   State_Invariant get_regval set_regval invariant inv_regs
   for CC :: "'cap Capability_class" and ISA :: "('cap, 'regval, 'instr, 'e) isa"
-    and translation_assm :: "'regval event list \<Rightarrow> bool"
+    and translation_assms :: "'regval event list \<Rightarrow> bool"
     and is_fetch :: bool and ex_traces :: bool
     and get_regval :: "string \<Rightarrow> 'regstate \<Rightarrow> 'regval option"
     and set_regval :: "string \<Rightarrow> 'regval \<Rightarrow> 'regstate \<Rightarrow> 'regstate option"
@@ -1615,7 +2166,7 @@ lemma traces_enabled_mem_axioms:
   assumes "traces_enabled m initial regs" and "hasTrace t m"
     and "reads_regs_from inv_regs t regs" and "invariant regs"
     and "hasException t m \<or> hasFailure t m \<longrightarrow> ex_traces"
-    and "translation_assm t"
+    and "translation_assms t"
   shows "store_mem_axiom CC ISA t"
     and "store_tag_axiom CC ISA t"
     and "load_mem_axiom CC ISA is_fetch t"
@@ -1686,7 +2237,7 @@ lemma non_cap_exp_trace_enabledI:
      (auto intro: non_cap_trace_enabledI simp: trace_enabled_append_iff)
 
 lemma accepts_iff_store_mem_tag_axioms:
-  assumes "translation_assm t"
+  assumes "translation_assms t"
   shows "accepts t \<longleftrightarrow> store_mem_axiom CC ISA t \<and> store_tag_axiom CC ISA t"
 proof
   assume *: "accepts t"
@@ -1714,7 +2265,7 @@ next
 qed
 
 lemma recognises_store_mem_tag_axioms:
-  assumes "translation_assm t" and "accepts t"
+  assumes "translation_assms t" and "accepts t"
   shows "store_mem_axiom CC ISA t" and "store_tag_axiom CC ISA t"
   using assms(2)
   unfolding accepts_iff_store_mem_tag_axioms[OF assms(1)]
@@ -1801,7 +2352,7 @@ lemma non_cap_exp_trace_enabledI:
      (auto intro: non_cap_trace_enabledI simp: trace_enabled_append_iff)
 
 lemma recognises_load_mem_axiom:
-  assumes "translation_assm t"
+  assumes "translation_assms t"
   shows "accepts t \<longleftrightarrow> load_mem_axiom CC ISA is_fetch t"
 proof
   assume *: "accepts t"
